proof/heap.bpl
@@ -1,12 +1,223 @@
-procedure L_malloc( size: uint64_t )
-//returns (result: uint8_ptr_t)
-//modifies mem;
-{
+/**
+ * Implements send and recv API
+ * Channel state from 0x1000 to 0x2000
+ */
 
+ type heap_api_result_t;
+ const unique heap_success: heap_api_result_t;
+ const unique heap_failure: heap_api_result_t;
+
+/*
+typedef struct {
+  uint8_t *heap_buf_start;
+  uint64_t heap_buf_size;
+  uint8_t *heap_buf_current;
+} sir_memory_context_t;
+*/
+
+type{:datatype} sir_heap_context_t;
+function{:constructor} sir_heap_context_t( heap_buf_start: uint8_ptr_t,
+                                           heap_buf_size: uint64_t,
+                                           heap_buf_current: uint8_ptr_t ) :
+                       sir_heap_context_t;
+
+/*
+typedef struct header {
+    struct header *ptr; // next block if on free list
+    uint64_t size;      // size of this block
+} malloc_header_t;
+*/
+type{:datatype} malloc_header_t;
+function{:constructor} malloc_header_t( ptr : header_ptr_t,
+                                        size: uint64_t ) :
+                       malloc_header_t;
+
+procedure {:inline 1} write_heap_context(ctx: sir_heap_context_t)
+modifies sir_heap_context;
+{
+  sir_heap_context := STORE_LE_64(sir_heap_context,
+                                    PLUS_64(sir_heap_context_ptr_low, 0bv64),
+                                    heap_buf_start#sir_heap_context_t(ctx));
+  sir_heap_context := STORE_LE_64(sir_heap_context,
+                                    PLUS_64(sir_heap_context_ptr_low, 8bv64),
+                                    heap_buf_size#sir_heap_context_t(ctx));
+  sir_heap_context := STORE_LE_64(sir_heap_context,
+                                    PLUS_64(sir_heap_context_ptr_low, 16bv64),
+                                    heap_buf_current#sir_heap_context_t(ctx));
 }
 
-procedure L_free( buf: uint8_ptr_t )
-//modifies mem;
+procedure {:inline 1} init_heap ( heap_buf_start: uint8_ptr_t,
+                                  heap_buf_size: uint64_t )
+modifies sir_heap_context, freep;
 {
+  var tmp: sir_heap_context_t;
+  tmp  :=  sir_heap_context_t ( heap_buf_start,
+                                heap_buf_size,
+                                heap_buf_start);
+  call write_heap_context(tmp);
+  freep := NULL;
+}
 
+procedure {:inline 1} bytes_available_in_heap_buf (size: uint64_t)
+returns (result: bool)
+requires AddrInHeap(LOAD_LE_64(sir_heap_context,
+                               PLUS_64(sir_heap_context_ptr_low, 16bv64)));
+{
+  var heap_buf_current: uint8_ptr_t;
+  var heap_buf_size: uint8_ptr_t;
+  var heap_buf_start: uint8_ptr_t;
+
+  heap_buf_start   := LOAD_LE_64(sir_heap_context,
+                                 PLUS_64(sir_heap_context_ptr_low, 0bv64));
+  heap_buf_size    := LOAD_LE_64(sir_heap_context,
+                                 PLUS_64(sir_heap_context_ptr_low, 8bv64));
+  heap_buf_current := LOAD_LE_64(sir_heap_context,
+                                 PLUS_64(sir_heap_context_ptr_low, 16bv64));
+
+  result := LE_64(PLUS_64(heap_buf_current, size), PLUS_64(heap_buf_start, heap_buf_size)) &&
+            GE_64(PLUS_64(heap_buf_current, size), heap_buf_current);
+  assert result ==>
+         (AddrInHeap(heap_buf_current) &&
+          AddrInHeap(PLUS_64(heap_buf_current, MINUS_64(size,1bv64))));
+}
+
+procedure {:inline 1} morecore( nunits: uint64_t )
+returns (result: header_ptr_t)
+modifies heap, sir_heap_context, freep;
+{
+  var nbytes: uint64_t;
+  var heap_buf_current: uint8_ptr_t;
+  var bytes_available: bool;
+  var free_api_result: heap_api_result_t;
+
+  heap_buf_current := LOAD_LE_64(sir_heap_context,
+                                 PLUS_64(sir_heap_context_ptr_low, 16bv64));
+  nbytes := LSHIFT_64(nunits, 4bv64);
+  call bytes_available := bytes_available_in_heap_buf( nbytes );
+  if (bytes_available)
+  {
+    result := heap_buf_current;
+    heap := STORE_LE_64(heap, PLUS_64(result, 8bv64), nunits);
+    call free_api_result := L_free(PLUS_64(result, 8bv64));
+    sir_heap_context := STORE_LE_64(sir_heap_context,
+                                    PLUS_64(sir_heap_context_ptr_low, 16bv64),
+                                    nbytes);
+  }
+  else { result := NULL; return; }
+}
+
+procedure L_malloc( size: uint64_t )
+returns (result: heap_api_result_t, region: virtual_addr_t)
+modifies heap, heap_base, freep, sir_heap_context;
+{
+  var p, p_ptr: header_ptr_t;
+  var prevp: header_ptr_t;
+  var return_flag : bool;
+  var nunits: uint64_t;
+  var p_size: uint64_t;
+
+  nunits := RSHIFT_64(nunits, 4bv64);
+
+  prevp := freep;
+  if (prevp == NULL)
+  {
+    prevp := heap_base_ptr_low;
+    freep := prevp;
+    heap_base := STORE_LE_64(heap_base,
+                             PLUS_64(heap_base_ptr_low, 0bv64),
+                             freep);
+    heap_base := STORE_LE_64(heap_base,
+                             PLUS_64(heap_base_ptr_low, 8bv64),
+                             freep);
+  }
+
+  p := LOAD_LE_64(heap, PLUS_64(prevp,0bv64));
+  return_flag := false;
+
+  while(!return_flag) {
+    p_ptr  := LOAD_LE_64(heap, PLUS_64(p, 0bv64)); //p->s.ptr
+    p_size := LOAD_LE_64(heap, PLUS_64(p, 8bv64)); //p->s.size
+    if (GE_64(p_size, nunits)) {
+      if (p_size == nunits) {
+        //prevp->s.ptr = p->s.ptr;
+        heap := STORE_LE_64(heap, PLUS_64(prevp, 0bv64), p_ptr);
+      } else {
+        heap := STORE_LE_64(heap, PLUS_64(p, 8bv64), MINUS_64(p_size,nunits));
+        p := PLUS_64(p, MINUS_64(p_size,nunits));
+        heap := STORE_LE_64(heap, PLUS_64(p, 8bv64), nunits);
+      }
+
+      freep := prevp;
+      region := PLUS_64(p, 16bv64); result := heap_success;
+      return_flag := true;
+    }
+    if (p == freep) {
+      call p := morecore(nunits);
+      if (p == NULL) {
+        region := NULL; result := heap_failure;
+        return_flag := true;
+      }
+    }
+    prevp := p;
+    p := p_ptr;
+  }
+  return;
+}
+
+procedure L_free( ap: uint8_ptr_t )
+returns (result: heap_api_result_t)
+modifies heap, freep;
+{
+  var bp, bp_ptr: header_ptr_t;
+  var p, p_ptr : header_ptr_t;
+  var p_size, bp_size: bv64;
+  var break_flag : bool;
+
+  bp := MINUS_64(ap, 16bv64);
+  p := freep;
+  break_flag := false;
+
+  while (!break_flag && !( GT_64(bp,p) && LT_64(bp, p_ptr) ))
+  {
+    p_ptr := LOAD_LE_64(heap, PLUS_64(p, 0bv64)); //p->s.ptr
+    if (GE_64(p,p_ptr) && (GT_64(bp,p) || LT_64(bp, p_ptr)))
+    {
+      break_flag := true;
+    }
+
+    p := p_ptr; //for(..; p = p->s.ptr)
+  }
+
+  p_ptr  := LOAD_LE_64(heap, PLUS_64(p, 0bv64)); //p->s.ptr
+  p_size := LOAD_LE_64(heap, PLUS_64(p, 8bv64)); //p->s.size
+  bp_ptr  := LOAD_LE_64(heap, PLUS_64(bp, 0bv64)); //p->s.ptr
+  bp_size := LOAD_LE_64(heap, PLUS_64(bp, 8bv64)); //p->s.size
+
+  if (PLUS_64(bp, bp_size) == p_ptr) {
+    heap := STORE_LE_64(heap,
+                        PLUS_64(bp, 8bv64),
+                        PLUS_64(bp_size, LOAD_LE_64(heap, PLUS_64(p_ptr, 8bv64))));
+    heap := STORE_LE_64(heap,
+                        PLUS_64(bp, 0bv64),
+                        LOAD_LE_64(heap, PLUS_64(p_ptr, 0bv64)));
+  } else {
+    heap := STORE_LE_64(heap,
+                        PLUS_64(bp, 0bv64),
+                        p_ptr);
+  }
+
+  if (PLUS_64(p, p_size) == bp_ptr) {
+    heap := STORE_LE_64(heap,
+                        PLUS_64(p, 8bv64),
+                        PLUS_64(p_size, LOAD_LE_64(heap, PLUS_64(bp_ptr, 8bv64))));
+    heap := STORE_LE_64(heap,
+                        PLUS_64(p, 0bv64),
+                        LOAD_LE_64(heap, PLUS_64(bp_ptr, 0bv64)));
+  } else {
+    heap := STORE_LE_64(heap,
+                        PLUS_64(p, 0bv64),
+                        bp);
+  }
+
+  freep := p;
 }
