proof/verified_L.bpl
@@ -1,9 +1,12 @@
 procedure main()
-modifies send_buf, recv_buf, stack, stack_guard, sir_channel_context, symmetric_key, U;
+modifies send_buf, recv_buf, stack, stack_guard, freep, sir_heap_context,
+         sir_channel_context, symmetric_key, U, heap, heap_base;
 {
   var buf: uint8_ptr_t;
   var size: uint64_t;
   var channel_result : channel_api_result_t;
+  var heap_result : heap_api_result_t;
+  var malloc_region : uint8_ptr_t;
 
   call init_channel(send_buf_ptr_low, send_buf_size,
                     recv_buf_ptr_low, recv_buf_size,
@@ -11,14 +14,18 @@ modifies send_buf, recv_buf, stack, stack_guard, sir_channel_context, symmetric_
 
   while(*)
   invariant AddrInSendBuf(LOAD_LE_64(sir_channel_context, PLUS_64(sir_channel_context_ptr_low, 16bv64)));
+  invariant LOAD_LE_64(sir_channel_context,
+                       PLUS_64(sir_channel_context_ptr_low, 8bv64)) == send_buf_size;
+  invariant LOAD_LE_64(sir_channel_context,
+                       PLUS_64(sir_channel_context_ptr_low, 0bv64)) == send_buf_ptr_low;
   {
     havoc buf;
     havoc size;
 
     if (*) { call U(); }
-    //else if (*) { call L_malloc(size); }
-    //else if (*) { call L_free(buf); }
+    else if (*) { call heap_result, malloc_region := L_malloc(size); }
+    else if (*) { call heap_result := L_free(buf); }
     else if (*) { call channel_result := L_send(buf,size); }
-    //else if (*) { call channel_result := L_recv(buf,size); }
+    else if (*) { call channel_result := L_recv(buf,size); }
   }
 }
